src/HOL/SPARK/Examples/RIPEMD-160/F.thy
@@ -26,7 +26,7 @@ spark_vc function_f_6
 proof -
   from H8 have "nat j <= 15" by simp
   with assms show ?thesis
-    by (simp add: f_def bwsimps int_word_uint take_bit_int_eq_self)
+    by (simp add: f_def bwsimps take_bit_int_eq_self)
 qed
 
 spark_vc function_f_7
@@ -34,7 +34,7 @@ proof -
   from H7 have "16 <= nat j" by simp
   moreover from H8 have "nat j <= 31" by simp
   ultimately show ?thesis using assms
-    by (simp only: f_def bwsimps int_word_uint)
+    by (simp only: f_def bwsimps)
       (simp add: take_bit_int_eq_self take_bit_not_eq_mask_diff mask_eq_exp_minus_1)
 qed
 
@@ -43,7 +43,7 @@ proof -
   from H7 have "32 <= nat j" by simp
   moreover from H8 have "nat j <= 47" by simp
   ultimately show ?thesis using assms
-    by (simp only: f_def bwsimps int_word_uint) (simp add: take_bit_int_eq_self take_bit_not_eq_mask_diff mask_eq_exp_minus_1)
+    by (simp only: f_def bwsimps) (simp add: take_bit_int_eq_self take_bit_not_eq_mask_diff mask_eq_exp_minus_1)
 qed
 
 spark_vc function_f_9
@@ -51,7 +51,7 @@ proof -
   from H7 have "48 <= nat j" by simp
   moreover from H8 have   "nat j <= 63" by simp
   ultimately show ?thesis using assms
-    by (simp only: f_def bwsimps int_word_uint) (simp add: take_bit_int_eq_self take_bit_not_eq_mask_diff mask_eq_exp_minus_1)
+    by (simp only: f_def bwsimps) (simp add: take_bit_int_eq_self take_bit_not_eq_mask_diff mask_eq_exp_minus_1)
 qed
 
 spark_vc function_f_10
@@ -59,7 +59,7 @@ proof -
   from H2 have "nat j <= 79" by simp
   moreover from H12 have "64 <= nat j" by simp
   ultimately show ?thesis using assms
-    by (simp only: f_def bwsimps int_word_uint) (simp add: take_bit_int_eq_self take_bit_not_eq_mask_diff mask_eq_exp_minus_1)
+    by (simp only: f_def bwsimps) (simp add: take_bit_int_eq_self take_bit_not_eq_mask_diff mask_eq_exp_minus_1)
 qed
 
 spark_end
